Make interpreter less eager, add dynamic dispatch

shift-reset/interpreter/interpreter.v
@@ -1,135 +1,36 @@
-From Stdlib Require Import String ZArith.
+From Stdlib Require Import String Qcanon ZArith.
 From shift_reset.core Require Import syntax env kont loc tag val var.
-From shift_reset.interpreter Require Import ierror iheap imonad.
+From shift_reset.interpreter Require Import dispatch ierror iheap imonad unwrap.
 
 Local Open Scope string_scope.
-Local Open Scope Z_scope.
 Local Open Scope imonad_scope.
 Local Unset Elimination Schemes.
 
-Inductive iresult : Type :=
-| RReturn : val -> iresult
-| RShift : tag -> (val -> imonad iresult) -> metakont -> iresult
-| RControl : tag -> (val -> imonad iresult) -> metakont -> iresult
-| RRaise : exn -> iresult
-| RPerform : metakont -> eff -> iresult.
-
-Definition unwrap_RReturn (r : iresult) : imonad val :=
-  match r with
-  | RReturn v => imonad_pure v
-  | RShift tag _ _ => imonad_throw_error (Undelimited_shift tag)
-  | RControl tag _ _ => imonad_throw_error (Undelimited_control tag)
-  | RRaise exn => imonad_throw_error (Unhandled_exception exn)
-  | RPerform _ eff => imonad_throw_error (Unhandled_effect eff)
-  end.
-
-Definition unwrap_vint (v : val) : imonad Z :=
-  match v with
-  | VInt i => imonad_pure i
-  | _ => imonad_throw_error (Type_error "")
-  end.
-
-Definition unwrap_vbool (v : val) : imonad bool :=
-  match v with
-  | VBool b => imonad_pure b
-  | _ => imonad_throw_error (Type_error "")
-  end.
-
-Definition unwrap_vref (v : val) : imonad loc :=
-  match v with
-  | VRef l => imonad_pure l
-  | _ => imonad_throw_error (Type_error "")
-  end.
-
-Definition unwrap_vprod (v : val) : imonad (val * val) :=
-  match v with
-  | VPair v1 v2 => imonad_pure (v1, v2)
-  | _ => imonad_throw_error (Type_error "")
-  end.
-
-Definition unwrap_vsum (v : val) : imonad (val + val) :=
-  match v with
-  | VInl v' => imonad_pure (inl v')
-  | VInr v' => imonad_pure (inr v')
-  | _ => imonad_throw_error (Type_error "")
-  end.
-
-Definition unwrap_vexn (v : val) : imonad exn :=
-  match v with
-  | VExn exn => imonad_pure exn
-  | _ => imonad_throw_error (Type_error "")
-  end.
-
-Definition unwrap_veff (v : val) : imonad eff :=
-  match v with
-  | VEff eff => imonad_pure eff
-  | _ => imonad_throw_error (Type_error "")
-  end.
-
-Definition interpret_i2i (f : Z -> Z) (m : imonad val) : imonad val :=
-  imonad_map (fun i => VInt (f i)) (m >>= unwrap_vint).
-
-Definition interpret_b2b (f : bool -> bool) (m : imonad val) : imonad val :=
-  imonad_map (fun b => VBool (f b)) (m >>= unwrap_vbool).
-
-Definition interpret_prim1 (p : prim1) : imonad val -> imonad val :=
-  match p with
-  | P1Neg => interpret_i2i Z.opp
-  | P1Not => interpret_b2b negb
-  end.
-
-Definition interpret_ii2i (f : Z -> Z -> Z) (m1 m2 : imonad val) : imonad val :=
-  imonad_lift2 (fun i1 i2 => VInt (f i1 i2)) (m1 >>= unwrap_vint) (m2 >>= unwrap_vint).
-
-Definition interpret_ii2b (f : Z -> Z -> bool) (m1 m2 : imonad val) : imonad val :=
-  imonad_lift2 (fun i1 i2 => VBool (f i1 i2)) (m1 >>= unwrap_vint) (m2 >>= unwrap_vint).
-
-Definition interpret_bb2b (f : bool -> bool -> bool) (m1 m2 : imonad val) : imonad val :=
-  imonad_lift2 (fun b1 b2 => VBool (f b1 b2)) (m1 >>= unwrap_vbool) (m2 >>= unwrap_vbool).
-
-Definition interpret_vv2b (f : val -> val -> bool) : imonad val -> imonad val -> imonad val :=
-  imonad_lift2 (fun v1 v2 => VBool (f v1 v2)).
-
-Definition interpret_prim2 (p : prim2) : imonad val -> imonad val -> imonad val :=
-  match p with
-  | P2Add => interpret_ii2i Z.add
-  | P2Sub => interpret_ii2i Z.sub
-  | P2Mul => interpret_ii2i Z.mul
-  | P2Div => interpret_ii2i Z.div
-  | P2Rem => interpret_ii2i Z.rem
-  | P2Lt => interpret_ii2b Z.ltb
-  | P2Le => interpret_ii2b Z.leb
-  | P2Gt => interpret_ii2b Z.gtb
-  | P2Ge => interpret_ii2b Z.geb
-  | P2And => interpret_bb2b andb
-  | P2Or => interpret_bb2b orb
-  | P2Xor => interpret_bb2b xorb
-  | P2Eq => interpret_vv2b val_eqb
-  | P2Neq => interpret_vv2b val_neqb
-  end.
-
 Fixpoint interpret_val_term (t : val_term) : imonad val :=
   match t with
-  | TVAtom a =>
-      match a with
-      | AUnit => imonad_pure VUnit
-      | AInt i => imonad_pure (VInt i)
-      | ABool b => imonad_pure (VBool b)
-      | AVar x =>
-          env <- imonad_ask_env;
-          match env_lookup x env with
-          | None => imonad_throw_error (Name_error x)
-          | Some v => imonad_pure v
-          end
+  | TVVar x =>
+      env <- imonad_ask_env;
+      match env_lookup x env with
+      | None => imonad_throw_error (Name_error x)
+      | Some v => imonad_pure v
       end
+  | TVUnit => imonad_pure VUnit
+  | TVInt z => imonad_pure (VInt z)
+  | TVFloat q => imonad_pure (VFloat q)
+  | TVNeg t' => interpret_val_term t' >>= dispatch_neg
+  | TVAdd t1 t2 => v <- interpret_val_term t1; f <- dispatch_add v; interpret_val_term t2 >>= f
+  | TVSub t1 t2 => v <- interpret_val_term t1; f <- dispatch_sub v; interpret_val_term t2 >>= f
+  | TVMul t1 t2 => v <- interpret_val_term t1; f <- dispatch_mul v; interpret_val_term t2 >>= f
+  | TVDiv t1 t2 => v <- interpret_val_term t1; f <- dispatch_div v; interpret_val_term t2 >>= f
+  | TVMod t1 t2 => v <- interpret_val_term t1; f <- dispatch_mod v; interpret_val_term t2 >>= f
+  | TVTrue => imonad_pure VTrue
+  | TVFalse => imonad_pure VFalse
+  | TVNot t' => interpret_val_term t' >>= dispatch_not
+  | TVAnd t1 t2 => v <- interpret_val_term t1; b <- unwrap_vbool v; if b then interpret_val_term t2 else imonad_pure v
+  | TVOr t1 t2 => v <- interpret_val_term t1; b <- unwrap_vbool v; if b then imonad_pure v else interpret_val_term t2
   | TVFun t' => imonad_asks_env (VFun' t')
   | TVFix t' => imonad_asks_env (VFix' t')
-  | TVPrim1 p t' => interpret_prim1 p (interpret_val_term t')
-  | TVPrim2 p t1 t2 => interpret_prim2 p (interpret_val_term t1) (interpret_val_term t2)
-  | TVPair t1 t2 =>
-      v1 <- interpret_val_term t1;
-      v2 <- interpret_val_term t2;
-      imonad_pure (VPair v1 v2)
+  | TVPair t1 t2 => v <- interpret_val_term t1; VPair v <$> interpret_val_term t2
   | TVInl t' => VInl <$> interpret_val_term t'
   | TVInr t' => VInr <$> interpret_val_term t'
   | TVRef t' =>
@@ -170,65 +71,32 @@ Fixpoint interpret_val_term (t : val_term) : imonad val :=
       v <- interpret_val_term t';
       b <- unwrap_vbool v;
       if b then imonad_pure VUnit else imonad_throw_error (Assert_failure "")
+  | TVLt t1 t2 => v <- interpret_val_term t1; f <- dispatch_lt v; interpret_val_term t2 >>= f
+  | TVLe t1 t2 => v <- interpret_val_term t1; f <- dispatch_le v; interpret_val_term t2 >>= f
+  | TVGt t1 t2 => v <- interpret_val_term t1; f <- dispatch_gt v; interpret_val_term t2 >>= f
+  | TVGe t1 t2 => v <- interpret_val_term t1; f <- dispatch_ge v; interpret_val_term t2 >>= f
+  | TVEq t1 t2 => v <- interpret_val_term t1; f <- dispatch_eq v; interpret_val_term t2 >>= f
+  | TVNeq t1 t2 => v <- interpret_val_term t1; f <- dispatch_neq v; interpret_val_term t2 >>= f
   end.
 
-Print interpret_val_term.
+Inductive iresult : Type :=
+| RVal : val -> iresult
+| RShift : metakont -> (val -> imonad iresult) -> tag -> iresult
+| RControl : metakont -> (val -> imonad iresult) -> tag -> iresult
+| RRaise : exn -> iresult
+| RPerform : metakont -> eff -> iresult.
 
 Fixpoint delimit_reset (tag : tag) (r : iresult) : imonad iresult :=
   match r with
-  | RShift tag' f mk => if tag_eq_dec tag tag' then f (VKontReset mk tag) >>= delimit_reset tag else imonad_pure r
+  | RShift mk f tag' => if tag_eqb tag tag' then f (VMKReset mk tag) >>= delimit_reset tag else imonad_pure r
   | _ => imonad_pure r
   end.
 
 Fixpoint delimit_prompt (tag : tag) (r : iresult) : imonad iresult :=
   match r with
-  | RControl tag' f mk => if tag_eq_dec tag tag' then f (VKont mk) >>= delimit_prompt tag else imonad_pure r
+  | RControl mk f tag' => if tag_eqb tag tag' then f (VMKPure mk) >>= delimit_prompt tag else imonad_pure r
   | _ => imonad_pure r
   end.
-
-Fixpoint unwind_reset (tag : tag) (k : kont) (f : val -> imonad iresult) (r : iresult) : imonad iresult :=
-  match r with
-  | RReturn v => f v
-  | RShift tag' f' mk =>
-      if tag_eq_dec tag tag'
-      then f' (VKontReset mk tag) >>= unwind_reset tag k f
-      else imonad_pure (RShift tag' f' (MKReset mk tag k))
-  | RControl tag' f' mk => imonad_pure (RControl tag' f' (MKReset mk tag k))
-  | RRaise _ => imonad_pure r
-  | RPerform mk eff => imonad_pure (RPerform (MKReset mk tag k) eff)
-  end.
-
-Fixpoint unwind_prompt (tag : tag) (k : kont) (f : val -> imonad iresult) (r : iresult) : imonad iresult :=
-  match r with
-  | RReturn v => f v
-  | RShift tag' f' mk => imonad_pure (RShift tag' f' (MKPrompt mk tag k))
-  | RControl tag' f' mk =>
-      if tag_eq_dec tag tag'
-      then f' (VKont mk) >>= unwind_prompt tag k f
-      else imonad_pure (RControl tag' f' (MKPrompt mk tag k))
-  | RRaise _ => imonad_pure r
-  | RPerform mk eff => imonad_pure (RPerform (MKPrompt mk tag k) eff)
-  end.
-
-Definition unwind_shallow_handle (k : kont) (c : handle_clo) (f : val -> imonad iresult) (h : eff -> val -> option (imonad iresult))
-  (r : iresult) : imonad iresult :=
-  match r with
-  | RReturn v => f v
-  | RShift tag f mk => imonad_pure (RShift tag f (MKShallowHandle mk c k))
-  | RControl tag f mk => imonad_pure (RControl tag f (MKShallowHandle mk c k))
-  | RRaise _ => imonad_pure r
-  | RPerform mk eff =>
-      match h eff (VKont mk) with
-      | Some m => m
-      | None => imonad_pure (RPerform (MKShallowHandle mk c k) eff)
-      end
-  end.
-
-Definition interpret_reset (k : kont) (tag : tag) (m : imonad iresult) (f : val -> imonad iresult) : imonad iresult :=
-  m >>= unwind_reset tag k f.
-
-Definition interpret_prompt (k : kont) (tag : tag) (m : imonad iresult) (f : val -> imonad iresult) : imonad iresult :=
-  m >>= unwind_prompt tag k f.
 
 Definition with_binder (b : binder) (v : val) (m : imonad iresult) : imonad iresult :=
   match b with
@@ -236,32 +104,33 @@ Definition with_binder (b : binder) (v : val) (m : imonad iresult) : imonad ires
   | BVar x => imonad_local_env (EnvCons x v) m
   end.
 
-(* TODO: rewrite this! *)
-Fixpoint match_exn (p : pattern) (exn : exn) (m : imonad iresult) : option (imonad iresult) :=
+Definition with_binder2 (b1 b2 : binder) (v1 v2 : val) (m : imonad iresult) : imonad iresult :=
+  with_binder b2 v2 (with_binder b1 v1 m).
+
+Fixpoint match_exn (p : pattern) (exn : exn) : option (imonad iresult -> imonad iresult) :=
   match p with
-  | PAny => Some m
-  | PVar x => Some (imonad_local_env (EnvCons x (VExn exn)) m)
+  | PAny => Some id
+  | PVar x => Some (imonad_local_env (EnvCons x (VExn exn)))
   | PConstr tag b =>
       let (tag', v) := exn in
-      if tag_eq_dec tag tag' then Some (with_binder b v m) else None
+      if tag_eqb tag tag' then Some (with_binder b v) else None
   | PAlias p' x =>
-      match match_exn p' exn m with
-      | Some m' => Some (imonad_local_env (EnvCons x (VExn exn)) m')
+      match match_exn p' exn with
+      | Some f => Some (fun m => imonad_local_env (EnvCons x (VExn exn)) (f m))
       | None => None
       end
   end.
 
-(* TODO: rewrite this! *)
-Fixpoint match_eff (p : pattern) (b : binder) (eff : eff) (v : val) (m : imonad iresult) : option (imonad iresult) :=
+Fixpoint match_eff (p : pattern) (b : binder) (eff : eff) (v : val) : option (imonad iresult -> imonad iresult) :=
   match p with
-  | PAny => Some (with_binder b v m)
-  | PVar x => Some (imonad_local_env (EnvCons x (VEff eff)) (with_binder b v m))
+  | PAny => Some (with_binder b v)
+  | PVar x => Some (fun m => imonad_local_env (EnvCons x (VEff eff)) (with_binder b v m))
   | PConstr tag b' =>
       let (tag', v') := eff in
-      if tag_eq_dec tag tag' then Some (with_binder b' v' (with_binder b v m)) else None
+      if tag_eqb tag tag' then Some (with_binder2 b b' v v') else None
   | PAlias p' x =>
-      match match_eff p' b eff v m with
-      | Some m' => Some (imonad_local_env (EnvCons x (VEff eff)) m')
+      match match_eff p' b eff v with
+      | Some f => Some (fun m => imonad_local_env (EnvCons x (VEff eff)) (f m))
       | None => None
       end
   end.
@@ -272,138 +141,119 @@ Definition interpret_term1_with (self : interpreter) (k : kont) (t : term1) (v :
   let (b, t') := t in with_binder b v (self k t').
 
 Definition interpret_term2_with (self : interpreter) (k : kont) (t : term2) (v1 v2 : val) : imonad iresult :=
-  let (b1, b2, t') := t in with_binder b1 v1 (with_binder b2 v2 (self k t')).
+  let (b1, b2, t') := t in with_binder2 b1 b2 v1 v2 (self k t').
 
-Definition interpret_clo1_with (self : interpreter) (k : kont) (c : clo1) (v : val) : imonad iresult :=
-  let (env, t) := c in imonad_use_env env (interpret_term1_with self k t v).
-
-Definition interpret_clo2_with (self : interpreter) (k : kont) (c : clo2) (v1 v2 : val) : imonad iresult :=
-  let (env, t) := c in imonad_use_env env (interpret_term2_with self k t v1 v2).
-
-Definition interpret_ctx_clo_with (self : interpreter) (k : kont) (c : ctx_clo) (v : val) : imonad iresult :=
+Definition interpret_kont_clo_with (self : interpreter) (k : kont) (c : kont_clo) (v : val) : imonad iresult :=
   match c with
-  | CCtx0 env t => imonad_use_env env (self k t)
-  | CCtx1 env t => imonad_use_env env (interpret_term1_with self k t v)
+  | CKSeq env t => imonad_use_env env (self k t)
+  | CKLet env t => imonad_use_env env (interpret_term1_with self k t v)
   end.
 
 Definition interpret_kont_with (self : interpreter) (k : kont) (v : val) : imonad iresult :=
   match k with
-  | KNil => imonad_pure (RReturn v)
-  | KCons c k' => interpret_ctx_clo_with self k' c v
+  | KNil => imonad_pure (RVal v)
+  | KCons c k' => interpret_kont_clo_with self k' c v
   end.
 
 Definition interpret_ret_term_with (self : interpreter) (k : kont) (t : ret_term) (v : val) : imonad iresult :=
   match t with
-  | TRet0 => interpret_kont_with self k v
-  | TRet1 b t' => with_binder b v (self k t')
+  | TRetNone => interpret_kont_with self k v
+  | TRetSome b t' => with_binder b v (self k t')
   end.
 
 Fixpoint interpret_exn_term_with (self : interpreter) (k : kont) (t : exn_term) (exn : exn) : option (imonad iresult) :=
   match t with
-  | TExnBase p t' => match_exn p exn (self k t') (* t' is executed eagerly, which is not good*)
+  | TExnLast p t' =>
+      match match_exn p exn with
+      | Some f => Some (f (self k t'))
+      | None => None
+      end
   | TExnCons p t1 t2 =>
-      let r := match_exn p exn (self k t1) in
-      (* t1 is executed eagerly *)
-      (* we need to "defer" the decision to execute t1 *)
-      match r with
-      | Some _ => r
+      match match_exn p exn with
+      | Some f => Some (f (self k t1))
       | None => interpret_exn_term_with self k t2 exn
       end
   end.
 
 Fixpoint interpret_eff_term_with (self : interpreter) (k : kont) (t : eff_term) (eff : eff) (v : val) : option (imonad iresult) :=
   match t with
-  | TEffBase p b t' => match_eff p b eff v (self k t') (* same problem as exn_term *)
+  | TEffLast p b t' =>
+      match match_eff p b eff v with
+      | Some f => Some (f (self k t'))
+      | None => None
+      end
   | TEffCons p b t1 t2 =>
-      let r := match_eff p b eff v (self k t1) in
-      match r with
-      | Some _ => r
+      match match_eff p b eff v with
+      | Some f => Some (f (self k t1))
       | None => interpret_eff_term_with self k t2 eff v
       end
   end.
 
-Definition interpret_try_clo_with (self : interpreter) (k : kont) (c : try_clo) (r : iresult) : imonad iresult :=
-  match r with
-  | RReturn v => interpret_kont_with self k v
-  | RShift tag f mk => imonad_pure (RShift tag f (MKTry mk c k))
-  | RControl tag f mk => imonad_pure (RControl tag f (MKTry mk c k))
-  | RRaise exn =>
-      let (env, t) := c in
-      match interpret_exn_term_with self k t exn with
-      | Some m => imonad_use_env env m
-      | None => imonad_pure r
-      end
-  | RPerform mk eff => imonad_pure (RPerform (MKTry mk c k) eff)
-  end.
-
-Definition interpret_handle_clo_with (self : interpreter) (k : kont) (c : handle_clo) (r : iresult) : imonad iresult :=
-  match r with
-  | RReturn v => let (env, t, _) := c in imonad_use_env env (interpret_ret_term_with self k t v)
-  | RShift tag f mk => imonad_pure (RShift tag f (MKHandle mk c k))
-  | RControl tag f mk => imonad_pure (RControl tag f (MKHandle mk c k))
-  | RRaise _ => imonad_pure r
-  | RPerform mk eff =>
-      let (env, _, t) := c in
-      match interpret_eff_term_with self k t eff (VKontHandle mk c) with
-      | Some m => imonad_use_env env m
-      | None => imonad_pure (RPerform (MKHandle mk c k) eff)
-      end
-  end.
-
-Definition interpret_shallow_handle_clo_with (self : interpreter) (k : kont) (c : handle_clo) : iresult -> imonad iresult :=
-  unwind_shallow_handle k c
-    (fun v =>
-       let (env, t, _) := c in
-       imonad_use_env env (interpret_ret_term_with self k t v))
-    (fun eff v =>
-       let (env, _, t) := c in
-       match interpret_eff_term_with self k t eff v with
-       | Some m => Some (imonad_use_env env m)
-       | None => None
-       end).
-
-(*match r with
-  | RReturn v => let (env, t, _) := c in imonad_use_env env (interpret_ret_term_with self k t v)
-  | RShift tag f mk => imonad_pure (RShift tag f (MKShallowHandle mk c k))
-  | RControl tag f mk => imonad_pure (RControl tag f (MKShallowHandle mk c k))
-  | RRaise _ => imonad_pure r
-  | RPerform mk eff =>
-      let (env, _, t) := c in
-      match interpret_eff_term_with self k t eff (VKont mk) with
-      | Some m => imonad_use_env env m
-      | None => imonad_pure (RPerform (MKShallowHandle mk c k) eff)
-      end
-  end.*)
-
 Fixpoint interpret_metakont_with (self : interpreter) (mk : metakont) (v : val) : imonad iresult :=
   match mk with
   | MKPure k => interpret_kont_with self k v
-  | MKReset mk' tag k => interpret_reset k tag (interpret_metakont_with self mk' v) (interpret_kont_with self k)
-  | MKPrompt mk' tag k => interpret_prompt k tag (interpret_metakont_with self mk' v) (interpret_kont_with self k)
-  | MKTry mk' c k => interpret_metakont_with self mk' v >>= interpret_try_clo_with self k c
-  | MKHandle mk' c k => interpret_metakont_with self mk' v >>= interpret_handle_clo_with self k c
-  | MKShallowHandle mk' c k => interpret_metakont_with self mk' v >>= interpret_shallow_handle_clo_with self k c
-  end.
-
-Definition interpret_app (self : interpreter) (k : kont) (m1 m2 : imonad val) (f : val -> imonad iresult) : imonad iresult :=
-  v <- m1;
-  match v with
-  | VFun c => m2 >>= interpret_clo1_with self k c
-  | VFix c => m2 >>= interpret_clo2_with self k c v
-  | VKontReset mk tag => interpret_reset k tag (m2 >>= interpret_metakont_with self mk) f
-  | VKont mk => m2 >>= interpret_metakont_with self (metakont_extend mk k)
-  | VKontHandle mk c => m2 >>= interpret_metakont_with self mk >>= interpret_handle_clo_with self k c
-  | _ => imonad_throw_error (Type_error "")
-  end.
-
-Definition unwrap_vcallable (self : interpreter) (k : kont) (v : val) (f : val -> imonad iresult) : imonad (val -> imonad iresult) :=
-  match v with
-  | VFun c => imonad_pure (interpret_clo1_with self k c)
-  | VFix c => imonad_pure (interpret_clo2_with self k c v)
-  | VKontReset mk tag => imonad_pure (interpret_metakont_with self mk >=> unwind_reset tag k f)
-  | VKont mk => imonad_pure (interpret_metakont_with self (metakont_extend mk k))
-  | VKontHandle mk c => imonad_pure (interpret_metakont_with self mk >=> interpret_handle_clo_with self k c)
-  | _ => imonad_throw_error (Type_error "")
+  | MKReset mk' tag k =>
+      r <- interpret_metakont_with self mk' v;
+      r <- delimit_reset tag r;
+      match r with
+      | RVal v => interpret_kont_with self k v
+      | RShift mk f tag' => imonad_pure (RShift (MKReset mk tag k) f tag')
+      | RControl mk f tag' => imonad_pure (RControl (MKReset mk tag k) f tag')
+      | RRaise _ => imonad_pure r
+      | RPerform mk eff => imonad_pure (RPerform (MKReset mk tag k) eff)
+      end
+  | MKPrompt mk' tag k =>
+      r <- interpret_metakont_with self mk' v;
+      r <- delimit_prompt tag r;
+      match r with
+      | RVal v => interpret_kont_with self k v
+      | RShift mk f tag' => imonad_pure (RShift (MKPrompt mk tag k) f tag')
+      | RControl mk f tag' => imonad_pure (RControl (MKPrompt mk tag k) f tag')
+      | RRaise _ => imonad_pure r
+      | RPerform mk eff => imonad_pure (RPerform (MKPrompt mk tag k) eff)
+      end
+  | MKTry mk' c k =>
+      r <- interpret_metakont_with self mk' v;
+      match r with
+      | RVal v => interpret_kont_with self k v
+      | RShift mk f tag => imonad_pure (RShift (MKTry mk c k) f tag)
+      | RControl mk f tag => imonad_pure (RControl (MKTry mk c k) f tag)
+      | RRaise exn =>
+          let (env, t) := c in
+          match interpret_exn_term_with self k t exn with
+          | Some m => imonad_use_env env m
+          | None => imonad_pure r
+          end
+      | RPerform mk eff => imonad_pure (RPerform (MKTry mk c k) eff)
+      end
+  | MKHandle mk' c k =>
+      r <- interpret_metakont_with self mk' v;
+      match r with
+      | RVal v => let (env, t, _) := c in imonad_use_env env (interpret_ret_term_with self k t v)
+      | RShift mk f tag => imonad_pure (RShift (MKHandle mk c k) f tag)
+      | RControl mk f tag => imonad_pure (RControl (MKHandle mk c k) f tag)
+      | RRaise _ => imonad_pure r
+      | RPerform mk eff =>
+          let (env, _, t) := c in
+          match interpret_eff_term_with self k t eff (VMKHandle mk c) with
+          | Some m => imonad_use_env env m
+          | None => imonad_pure (RPerform (MKHandle mk c k) eff)
+          end
+      end
+  | MKShallowHandle mk' c k =>
+      r <- interpret_metakont_with self mk' v;
+      match r with
+      | RVal v => let (env, t, _) := c in imonad_use_env env (interpret_ret_term_with self k t v)
+      | RShift mk f tag => imonad_pure (RShift (MKShallowHandle mk c k) f tag)
+      | RControl mk f tag => imonad_pure (RControl (MKShallowHandle mk c k) f tag)
+      | RRaise _ => imonad_pure r
+      | RPerform mk eff =>
+          let (env, _, t) := c in
+          match interpret_eff_term_with self k t eff (VMKPure mk) with
+          | Some m => imonad_use_env env m
+          | None => imonad_pure (RPerform (MKShallowHandle mk c k) eff)
+          end
+      end
   end.
 
 Set Implicit Arguments.
@@ -411,14 +261,14 @@ Set Implicit Arguments.
 Inductive term_graph : kont -> term -> Prop :=
 | GTVal k t' : kont_graph k -> term_graph k (TVal t')
 | GTApp k t1 t2 : kont_graph k -> term_graph k (TApp t1 t2)
-| GTLet k t1 t2 : (forall env, term_graph (KCons (CCtx1 env t2) k) t1) -> term_graph k (TLet t1 t2)
-| GTSeq k t1 t2 : (forall env, term_graph (KCons (CCtx0 env t2) k) t1) -> term_graph k (TSeq t1 t2)
+| GTSeq k t1 t2 : (forall env, term_graph (KCons (CKSeq env t2) k) t1) -> term_graph k (TSeq t1 t2)
+| GTLet k t1 t2 : (forall env, term_graph (KCons (CKLet env t2) k) t1) -> term_graph k (TLet t1 t2)
 | GTIf k t1 t2 t3 : term_graph k t2 -> term_graph k t3 -> term_graph k (TIf t1 t2 t3)
 | GTSplit k t1 t2 : term2_graph k t2 -> term_graph k (TSplit t1 t2)
 | GTCase k t1 t2 t3 : term1_graph k t2 -> term1_graph k t3 -> term_graph k (TCase t1 t2 t3)
-| GTShift k tag t' : (forall env, ctx_clo_graph KNil (CCtx1 env t')) -> term_graph k (TShift tag t')
+| GTShift k tag t' : term1_graph KNil t' -> term_graph k (TShift tag t')
 | GTReset k tag t' : term_graph KNil t' -> kont_graph k -> term_graph k (TReset tag t')
-| GTControl k tag t' : (forall env, ctx_clo_graph KNil (CCtx1 env t')) -> term_graph k (TControl tag t')
+| GTControl k tag t' : term1_graph KNil t' -> term_graph k (TControl tag t')
 | GTPrompt k tag t' : term_graph KNil t' -> kont_graph k -> term_graph k (TPrompt tag t')
 | GTRaise k t' : term_graph k (TRaise t')
 | GTTry k t1 t2 : term_graph KNil t1 -> kont_graph k -> exn_term_graph k t2 -> term_graph k (TTry t1 t2)
@@ -430,20 +280,20 @@ with term1_graph : kont -> term1 -> Prop :=
 with term2_graph : kont -> term2 -> Prop :=
 | GT2 k b1 b2 t' : term_graph k t' -> term2_graph k (T2 b1 b2 t')
 with ret_term_graph : kont -> ret_term -> Prop :=
-| GTRet0 k : kont_graph k -> ret_term_graph k TRet0
-| GTRet1 k b t' : term_graph k t' -> ret_term_graph k (TRet1 b t')
+| GTRetNone k : kont_graph k -> ret_term_graph k TRetNone
+| GTRetSome k b t' : term_graph k t' -> ret_term_graph k (TRetSome b t')
 with exn_term_graph : kont -> exn_term -> Prop :=
-| GTExnBase k p t' : term_graph k t' -> exn_term_graph k (TExnBase p t')
+| GTExnLast k p t' : term_graph k t' -> exn_term_graph k (TExnLast p t')
 | GTExnCons k p t1 t2 : term_graph k t1 -> exn_term_graph k t2 -> exn_term_graph k (TExnCons p t1 t2)
 with eff_term_graph : kont -> eff_term -> Prop :=
-| GTEffBase k p b t' : term_graph k t' -> eff_term_graph k (TEffBase p b t')
+| GTEffLast k p b t' : term_graph k t' -> eff_term_graph k (TEffLast p b t')
 | GTEffCons k p b t1 t2 : term_graph k t1 -> eff_term_graph k t2 -> eff_term_graph k (TEffCons p b t1 t2)
-with ctx_clo_graph : kont -> ctx_clo -> Prop :=
-| GCCtx0 k env t : term_graph k t -> ctx_clo_graph k (CCtx0 env t)
-| GCCtx1 k env t : term1_graph k t -> ctx_clo_graph k (CCtx1 env t)
+with kont_clo_graph : kont -> kont_clo -> Prop :=
+| GCKSeq k env t : term_graph k t -> kont_clo_graph k (CKSeq env t)
+| GCKLet k env t : term1_graph k t -> kont_clo_graph k (CKLet env t)
 with kont_graph : kont -> Prop :=
 | GKNil : kont_graph KNil
-| GKCons c k' : ctx_clo_graph k' c -> kont_graph (KCons c k').
+| GKCons c k' : kont_clo_graph k' c -> kont_graph (KCons c k').
 
 Lemma GTVal_inv k t' : term_graph k (TVal t') -> kont_graph k.
 Proof. inversion 1; auto. Defined.
@@ -451,10 +301,10 @@ Proof. inversion 1; auto. Defined.
 Lemma GTApp_inv k t1 t2 : term_graph k (TApp t1 t2) -> kont_graph k.
 Proof. inversion 1; auto. Defined.
 
-Lemma GTLet_inv k t1 t2 : term_graph k (TLet t1 t2) -> forall env, term_graph (KCons (CCtx1 env t2) k) t1.
+Lemma GTSeq_inv k t1 t2 : term_graph k (TSeq t1 t2) -> forall env, term_graph (KCons (CKSeq env t2) k) t1.
 Proof. inversion 1; auto. Defined.
 
-Lemma GTSeq_inv k t1 t2 : term_graph k (TSeq t1 t2) -> forall env, term_graph (KCons (CCtx0 env t2) k) t1.
+Lemma GTLet_inv k t1 t2 : term_graph k (TLet t1 t2) -> forall env, term_graph (KCons (CKLet env t2) k) t1.
 Proof. inversion 1; auto. Defined.
 
 Lemma GTIf_inv1 k t1 t2 t3 : term_graph k (TIf t1 t2 t3) -> term_graph k t2.
@@ -472,7 +322,7 @@ Proof. inversion 1; auto. Defined.
 Lemma GTCase_inv2 k t1 t2 t3 : term_graph k (TCase t1 t2 t3) -> term1_graph k t3.
 Proof. inversion 1; auto. Defined.
 
-Lemma GTShift_inv k tag t' : term_graph k (TShift tag t') -> forall env, ctx_clo_graph KNil (CCtx1 env t').
+Lemma GTShift_inv k tag t' : term_graph k (TShift tag t') -> term1_graph KNil t'.
 Proof. inversion 1; auto. Defined.
 
 Lemma GTReset_inv1 k tag t' : term_graph k (TReset tag t') -> term_graph KNil t'.
@@ -481,7 +331,7 @@ Proof. inversion 1; auto. Defined.
 Lemma GTReset_inv2 k tag t' : term_graph k (TReset tag t') -> kont_graph k.
 Proof. inversion 1; auto. Defined.
 
-Lemma GTControl_inv k tag t' : term_graph k (TControl tag t') -> forall env, ctx_clo_graph KNil (CCtx1 env t').
+Lemma GTControl_inv k tag t' : term_graph k (TControl tag t') -> term1_graph KNil t'.
 Proof. inversion 1; auto. Defined.
 
 Lemma GTPrompt_inv1 k tag t' : term_graph k (TPrompt tag t') -> term_graph KNil t'.
@@ -523,13 +373,13 @@ Proof. inversion 1; auto. Defined.
 Lemma GT2_inv k b1 b2 t' : term2_graph k (T2 b1 b2 t') -> term_graph k t'.
 Proof. inversion 1; auto. Defined.
 
-Lemma GTRet0_inv k : ret_term_graph k TRet0 -> kont_graph k.
+Lemma GTRetNone_inv k : ret_term_graph k TRetNone -> kont_graph k.
 Proof. inversion 1; auto. Defined.
 
-Lemma GTRet1_inv k b t' : ret_term_graph k (TRet1 b t') -> term_graph k t'.
+Lemma GTRetSome_inv k b t' : ret_term_graph k (TRetSome b t') -> term_graph k t'.
 Proof. inversion 1; auto. Defined.
 
-Lemma GTExnBase_inv k p t' : exn_term_graph k (TExnBase p t') -> term_graph k t'.
+Lemma GTExnLast_inv k p t' : exn_term_graph k (TExnLast p t') -> term_graph k t'.
 Proof. inversion 1; auto. Defined.
 
 Lemma GTExnCons_inv1 k p t1 t2 : exn_term_graph k (TExnCons p t1 t2) -> term_graph k t1.
@@ -538,7 +388,7 @@ Proof. inversion 1; auto. Defined.
 Lemma GTExnCons_inv2 k p t1 t2 : exn_term_graph k (TExnCons p t1 t2) -> exn_term_graph k t2.
 Proof. inversion 1; auto. Defined.
 
-Lemma GTEffBase_inv k p b t' : eff_term_graph k (TEffBase p b t') -> term_graph k t'.
+Lemma GTEffLast_inv k p b t' : eff_term_graph k (TEffLast p b t') -> term_graph k t'.
 Proof. inversion 1; auto. Defined.
 
 Lemma GTEffCons_inv1 k p b t1 t2 : eff_term_graph k (TEffCons p b t1 t2) -> term_graph k t1.
@@ -547,27 +397,27 @@ Proof. inversion 1; auto. Defined.
 Lemma GTEffCons_inv2 k p b t1 t2 : eff_term_graph k (TEffCons p b t1 t2) -> eff_term_graph k t2.
 Proof. inversion 1; auto. Defined.
 
-Lemma GCCtx0_inv k env t : ctx_clo_graph k (CCtx0 env t) -> term_graph k t.
+Lemma GCKSeq_inv k env t : kont_clo_graph k (CKSeq env t) -> term_graph k t.
 Proof. inversion 1; auto. Defined.
 
-Lemma GCCtx1_inv k env t : ctx_clo_graph k (CCtx1 env t) -> term1_graph k t.
+Lemma GCKLet_inv k env t : kont_clo_graph k (CKLet env t) -> term1_graph k t.
 Proof. inversion 1; auto. Defined.
 
-Lemma GKCons_inv c k' : kont_graph (KCons c k') -> ctx_clo_graph k' c.
+Lemma GKCons_inv c k' : kont_graph (KCons c k') -> kont_clo_graph k' c.
 Proof. inversion 1; auto. Defined.
 
 Fixpoint build_term_graph_dep (k : kont) (G : kont_graph k) (t : term) : term_graph k t :=
   match t with
   | TVal t' => GTVal t' G
   | TApp t1 t2 => GTApp t1 t2 G
-  | TLet t1 t2 => GTLet (fun env => build_term_graph_dep (GKCons (GCCtx1 env (build_term1_graph_dep G t2))) t1)
-  | TSeq t1 t2 => GTSeq (fun env => build_term_graph_dep (GKCons (GCCtx0 env (build_term_graph_dep G t2))) t1)
+  | TSeq t1 t2 => GTSeq (fun env => build_term_graph_dep (GKCons (GCKSeq env (build_term_graph_dep G t2))) t1)
+  | TLet t1 t2 => GTLet (fun env => build_term_graph_dep (GKCons (GCKLet env (build_term1_graph_dep G t2))) t1)
   | TIf t1 t2 t3 => GTIf t1 (build_term_graph_dep G t2) (build_term_graph_dep G t3)
   | TSplit t1 t2 => GTSplit t1 (build_term2_graph_dep G t2)
   | TCase t1 t2 t3 => GTCase t1 (build_term1_graph_dep G t2) (build_term1_graph_dep G t3)
-  | TShift tag t' => GTShift k tag (fun env => GCCtx1 env (build_term1_graph_dep GKNil t'))
+  | TShift tag t' => GTShift k tag (build_term1_graph_dep GKNil t')
   | TReset tag t' => GTReset tag (build_term_graph_dep GKNil t') G
-  | TControl tag t' => GTControl k tag (fun env => GCCtx1 env (build_term1_graph_dep GKNil t'))
+  | TControl tag t' => GTControl k tag (build_term1_graph_dep GKNil t')
   | TPrompt tag t' => GTPrompt tag (build_term_graph_dep GKNil t') G
   | TRaise t' => GTRaise k t'
   | TTry t1 t2 => GTTry (build_term_graph_dep GKNil t1) G (build_exn_term_graph_dep G t2)
@@ -576,53 +426,70 @@ Fixpoint build_term_graph_dep (k : kont) (G : kont_graph k) (t : term) : term_gr
   | TShallowHandle t1 t2 t3 => GTShallowHandle (build_term_graph_dep GKNil t1) (build_ret_term_graph_dep G t2) (build_eff_term_graph_dep G t3)
   end
 with build_term1_graph_dep (k : kont) (G : kont_graph k) (t : term1) : term1_graph k t :=
-  match t with
-  | T1 b t' => GT1 b (build_term_graph_dep G t')
-  end
+  let 'T1 b t' := t in GT1 b (build_term_graph_dep G t')
 with build_term2_graph_dep (k : kont) (G : kont_graph k) (t : term2) : term2_graph k t :=
-  match t with
-  | T2 b1 b2 t' => GT2 b1 b2 (build_term_graph_dep G t')
-  end
+  let 'T2 b1 b2 t' := t in GT2 b1 b2 (build_term_graph_dep G t')
 with build_ret_term_graph_dep (k : kont) (G : kont_graph k) (t : ret_term) : ret_term_graph k t :=
   match t with
-  | TRet0 => GTRet0 G
-  | TRet1 b t' => GTRet1 b (build_term_graph_dep G t')
+  | TRetNone => GTRetNone G
+  | TRetSome b t' => GTRetSome b (build_term_graph_dep G t')
   end
 with build_exn_term_graph_dep (k : kont) (G : kont_graph k) (t : exn_term) : exn_term_graph k t :=
   match t with
-  | TExnBase p t' => GTExnBase p (build_term_graph_dep G t')
+  | TExnLast p t' => GTExnLast p (build_term_graph_dep G t')
   | TExnCons p t1 t2 => GTExnCons p (build_term_graph_dep G t1) (build_exn_term_graph_dep G t2)
   end
 with build_eff_term_graph_dep (k : kont) (G : kont_graph k) (t : eff_term) : eff_term_graph k t :=
   match t with
-  | TEffBase p b t' => GTEffBase p b (build_term_graph_dep G t')
+  | TEffLast p b t' => GTEffLast p b (build_term_graph_dep G t')
   | TEffCons p b t1 t2 => GTEffCons p b (build_term_graph_dep G t1) (build_eff_term_graph_dep G t2)
   end.
 
-Definition build_ctx_clo_graph_dep (k : kont) (G : kont_graph k) (c : ctx_clo) : ctx_clo_graph k c :=
+Definition build_kont_clo_graph_dep (k : kont) (G : kont_graph k) (c : kont_clo) : kont_clo_graph k c :=
   match c with
-  | CCtx0 env t => GCCtx0 env (build_term_graph_dep G t)
-  | CCtx1 env t => GCCtx1 env (build_term1_graph_dep G t)
+  | CKSeq env t => GCKSeq env (build_term_graph_dep G t)
+  | CKLet env t => GCKLet env (build_term1_graph_dep G t)
   end.
 
 Fixpoint interpret_term_dep (self : interpreter) (k : kont) (t : term) (G : term_graph k t) {struct G} : imonad iresult :=
-  match t return term_graph k t -> imonad iresult with
-  | TVal t' =>
-      fun G => interpret_val_term t' >>= interpret_kont_dep self (GTVal_inv G)
+  match t return term_graph k t -> _ with
+  | TVal t' => fun G => interpret_val_term t' >>= interpret_kont_dep self (GTVal_inv G)
   | TApp t1 t2 =>
       fun G =>
-        v <- interpret_val_term t1;
-        c <- unwrap_vcallable self k v (interpret_kont_dep self (GTApp_inv G));
+        u <- interpret_val_term t1;
+        l <- unwrap_vlambda u;
         v <- interpret_val_term t2;
-        c v
-  | TLet t1 t2 =>
-      fun G =>
-        env <- imonad_ask_env;
-        interpret_term_dep self (GTLet_inv G env)
-  | TSeq t1 t2 =>
-      fun G =>
-        env <- imonad_ask_env;
-        interpret_term_dep self (GTSeq_inv G env)
+        match l with
+        | LFun c => let (env, t) := c in imonad_use_env env (interpret_term1_with self k t v)
+        | LFix c => let (env, t) := c in imonad_use_env env (interpret_term2_with self k t u v)
+        | LMKPure mk => interpret_metakont_with self (metakont_extend mk k) v
+        | LMKReset mk tag =>
+            r <- interpret_metakont_with self mk v;
+            r <- delimit_reset tag r;
+            match r with
+            | RVal v => interpret_kont_dep self (GTApp_inv G) v
+            | RShift mk f tag' => imonad_pure (RShift (MKReset mk tag k) f tag')
+            | RControl mk f tag' => imonad_pure (RControl (MKReset mk tag k) f tag')
+            | RRaise _ => imonad_pure r
+            | RPerform mk eff => imonad_pure (RPerform (MKReset mk tag k) eff)
+            end
+        | LMKHandle mk c =>
+            r <- interpret_metakont_with self mk v;
+            match r with
+            | RVal v => let (env, t, _) := c in imonad_use_env env (interpret_ret_term_with self k t v)
+            | RShift mk f tag => imonad_pure (RShift (MKHandle mk c k) f tag)
+            | RControl mk f tag => imonad_pure (RControl (MKHandle mk c k) f tag)
+            | RRaise _ => imonad_pure r
+            | RPerform mk eff =>
+                let (env, _, t) := c in
+                match interpret_eff_term_with self k t eff (VMKHandle mk c) with
+                | Some m => imonad_use_env env m
+                | None => imonad_pure (RPerform (MKHandle mk c k) eff)
+                end
+            end
+        end
+  | TSeq t1 t2 => fun G => env <- imonad_ask_env; interpret_term_dep self (GTSeq_inv G env)
+  | TLet t1 t2 => fun G => env <- imonad_ask_env; interpret_term_dep self (GTLet_inv G env)
   | TIf t1 t2 t3 =>
       fun G =>
         v <- interpret_val_term t1;
@@ -642,43 +509,39 @@ Fixpoint interpret_term_dep (self : interpreter) (k : kont) (t : term) (G : term
         | inr v' => interpret_term1_dep self (GTCase_inv2 G) v
         end
   | TShift tag t' =>
-      fun G => imonad_asks_env (fun env => RShift tag (interpret_ctx_clo_dep self (GTShift_inv G env)) (MKPure k))
+      fun G => imonad_asks_env (fun env => RShift (MKPure k) (fun v => imonad_use_env env (interpret_term1_dep self (GTShift_inv G) v)) tag)
   | TReset tag t' =>
       fun G =>
         r <- interpret_term_dep self (GTReset_inv1 G);
         r <- delimit_reset tag r;
         match r with
-        | RReturn v => interpret_kont_dep self (GTReset_inv2 G) v
-        | RShift tag' f mk => imonad_pure (RShift tag' f (MKReset mk tag k))
-        | RControl tag' f mk => imonad_pure (RControl tag' f (MKReset mk tag k))
+        | RVal v => interpret_kont_dep self (GTReset_inv2 G) v
+        | RShift mk f tag' => imonad_pure (RShift (MKReset mk tag k) f tag')
+        | RControl mk f tag' => imonad_pure (RControl (MKReset mk tag k) f tag')
         | RRaise _ => imonad_pure r
         | RPerform mk eff => imonad_pure (RPerform (MKReset mk tag k) eff)
         end
   | TControl tag t' =>
-      fun G =>
-        imonad_asks_env (fun env => RShift tag (interpret_ctx_clo_dep self (GTControl_inv G env)) (MKPure k))
+      fun G => imonad_asks_env (fun env => RControl (MKPure k) (fun v => imonad_use_env env (interpret_term1_dep self (GTControl_inv G) v)) tag)
   | TPrompt tag t' =>
       fun G =>
         r <- interpret_term_dep self (GTPrompt_inv1 G);
         r <- delimit_prompt tag r;
         match r with
-        | RReturn v => interpret_kont_dep self (GTPrompt_inv2 G) v
-        | RShift tag' f mk => imonad_pure (RShift tag' f (MKPrompt mk tag k))
-        | RControl tag' f mk => imonad_pure (RControl tag' f (MKPrompt mk tag k))
+        | RVal v => interpret_kont_dep self (GTPrompt_inv2 G) v
+        | RShift mk f tag' => imonad_pure (RShift (MKPrompt mk tag k) f tag')
+        | RControl mk f tag' => imonad_pure (RControl (MKPrompt mk tag k) f tag')
         | RRaise _ => imonad_pure r
         | RPerform mk eff => imonad_pure (RPerform (MKPrompt mk tag k) eff)
         end
-  | TRaise t' =>
-      fun G =>
-        v <- interpret_val_term t';
-        RRaise <$> unwrap_vexn v
+  | TRaise t' => fun G => v <- interpret_val_term t'; RRaise <$> unwrap_vexn v
   | TTry t1 t2 =>
       fun G =>
         r <- interpret_term_dep self (GTTry_inv1 G);
         match r with
-        | RReturn v => interpret_kont_dep self (GTTry_inv2 G) v
-        | RShift tag f mk => imonad_asks_env (fun env => RShift tag f (MKTry' mk t2 k env))
-        | RControl tag f mk => imonad_asks_env (fun env => RControl tag f (MKTry' mk t2 k env))
+        | RVal v => interpret_kont_dep self (GTTry_inv2 G) v
+        | RShift mk f tag => imonad_asks_env (fun env => RShift (MKTry' mk t2 k env) f tag)
+        | RControl mk f tag => imonad_asks_env (fun env => RControl (MKTry' mk t2 k env) f tag)
         | RRaise exn =>
             match interpret_exn_term_dep self (GTTry_inv3 G) exn with
             | Some m => m
@@ -686,22 +549,19 @@ Fixpoint interpret_term_dep (self : interpreter) (k : kont) (t : term) (G : term
             end
         | RPerform mk eff => imonad_asks_env (fun env => RPerform (MKTry' mk t2 k env) eff)
         end
-  | TPerform t' =>
-      fun G =>
-        v <- interpret_val_term t';
-        RPerform (MKPure k) <$> unwrap_veff v
+  | TPerform t' => fun G => v <- interpret_val_term t'; RPerform (MKPure k) <$> unwrap_veff v
   | THandle t1 t2 t3 =>
       fun G =>
         r <- interpret_term_dep self (GTHandle_inv1 G);
         match r with
-        | RReturn v => interpret_ret_term_dep self (GTHandle_inv2 G) v
-        | RShift tag f mk => imonad_asks_env (fun env => RShift tag f (MKHandle' mk t2 t3 k env))
-        | RControl tag f mk => imonad_asks_env (fun env => RControl tag f (MKHandle' mk t2 t3 k env))
+        | RVal v => interpret_ret_term_dep self (GTHandle_inv2 G) v
+        | RShift mk f tag => imonad_asks_env (fun env => RShift (MKHandle' mk t2 t3 k env) f tag)
+        | RControl mk f tag => imonad_asks_env (fun env => RControl (MKHandle' mk t2 t3 k env) f tag)
         | RRaise _ => imonad_pure r
         | RPerform mk eff =>
             env <- imonad_ask_env;
             let c := CHandle env t2 t3 in
-            match interpret_eff_term_dep self (GTHandle_inv3 G) eff (VKontHandle mk c) with
+            match interpret_eff_term_dep self (GTHandle_inv3 G) eff (VMKHandle mk c) with
             | Some m => m
             | None => imonad_pure (RPerform (MKHandle mk c k) eff)
             end
@@ -710,67 +570,59 @@ Fixpoint interpret_term_dep (self : interpreter) (k : kont) (t : term) (G : term
       fun G =>
         r <- interpret_term_dep self (GTShallowHandle_inv1 G);
         match r with
-        | RReturn v => interpret_ret_term_dep self (GTShallowHandle_inv2 G) v
-        | RShift tag f mk => imonad_asks_env (fun env => RShift tag f (MKShallowHandle' mk t2 t3 k env))
-        | RControl tag f mk => imonad_asks_env (fun env => RControl tag f (MKShallowHandle' mk t2 t3 k env))
+        | RVal v => interpret_ret_term_dep self (GTShallowHandle_inv2 G) v
+        | RShift mk f tag => imonad_asks_env (fun env => RShift (MKShallowHandle' mk t2 t3 k env) f tag)
+        | RControl mk f tag => imonad_asks_env (fun env => RControl (MKShallowHandle' mk t2 t3 k env) f tag)
         | RRaise _ => imonad_pure r
         | RPerform mk eff =>
-            match interpret_eff_term_dep self (GTShallowHandle_inv3 G) eff (VKont mk) with
+            match interpret_eff_term_dep self (GTShallowHandle_inv3 G) eff (VMKPure mk) with
             | Some m => m
             | None => imonad_asks_env (fun env => RPerform (MKShallowHandle' mk t2 t3 k env) eff)
             end
         end
   end G
 with interpret_term1_dep (self : interpreter) (k : kont) (t : term1) (G : term1_graph k t) (v : val) {struct G} : imonad iresult :=
-  match t return term1_graph k t -> imonad iresult with
-  | T1 b t' => fun G => with_binder b v (interpret_term_dep self (GT1_inv G))
-  end G
+  (let 'T1 b t' := t return term1_graph k t -> _ in fun G => with_binder b v (interpret_term_dep self (GT1_inv G))) G
 with interpret_term2_dep (self : interpreter) (k : kont) (t : term2) (G : term2_graph k t) (v1 v2 : val) {struct G} : imonad iresult :=
-  match t return term2_graph k t -> imonad iresult with
-  | T2 b1 b2 t' => fun G => with_binder b1 v1 (with_binder b2 v2 (interpret_term_dep self (GT2_inv G)))
-  end G
+  (let 'T2 b1 b2 t' := t return term2_graph k t -> _ in fun G => with_binder2 b1 b2 v1 v2 (interpret_term_dep self (GT2_inv G))) G
 with interpret_ret_term_dep (self : interpreter) (k : kont) (t : ret_term) (G : ret_term_graph k t) (v : val) {struct G} : imonad iresult :=
-  match t return ret_term_graph k t -> imonad iresult with
-  | TRet0 => fun G => interpret_kont_dep self (GTRet0_inv G) v
-  | TRet1 b t' => fun G => with_binder b v (interpret_term_dep self (GTRet1_inv G))
+  match t return ret_term_graph k t -> _ with
+  | TRetNone => fun G => interpret_kont_dep self (GTRetNone_inv G) v
+  | TRetSome b t' => fun G => with_binder b v (interpret_term_dep self (GTRetSome_inv G))
   end G
 with interpret_exn_term_dep (self : interpreter) (k : kont) (t : exn_term) (G : exn_term_graph k t) (exn : exn) {struct G} :
   option (imonad iresult) :=
-  match t return exn_term_graph k t -> option (imonad iresult) with
-  | TExnBase p t' =>
-      fun G =>
-        match_exn p exn (interpret_term_dep self (GTExnBase_inv G))
-  | TExnCons p t1 t2 =>
-      fun G =>
-        let r := match_exn p exn (interpret_term_dep self (GTExnCons_inv1 G)) in
-        match r with
-        | Some _ => r
-        | None => interpret_exn_term_dep self (GTExnCons_inv2 G) exn
-        end
+  match t return exn_term_graph k t -> _ with
+  | TExnLast p t' => fun G => match match_exn p exn with
+                              | Some f => Some (f (interpret_term_dep self (GTExnLast_inv G)))
+                              | None => None
+                              end
+  | TExnCons p t1 t2 => fun G => match match_exn p exn with
+                                 | Some f => Some (f (interpret_term_dep self (GTExnCons_inv1 G)))
+                                 | None => interpret_exn_term_dep self (GTExnCons_inv2 G) exn
+                                 end
   end G
 with interpret_eff_term_dep (self : interpreter) (k : kont) (t : eff_term) (G : eff_term_graph k t) (eff : eff) (v : val) {struct G} :
   option (imonad iresult) :=
-  match t return eff_term_graph k t -> option (imonad iresult) with
-  | TEffBase p b t' =>
-      fun G =>
-        match_eff p b eff v (interpret_term_dep self (GTEffBase_inv G))
-  | TEffCons p b t1 t2 =>
-      fun G =>
-        let r := match_eff p b eff v (interpret_term_dep self (GTEffCons_inv1 G)) in
-        match r with
-        | Some _ => r
-        | None => interpret_eff_term_dep self (GTEffCons_inv2 G) eff v
-        end
+  match t return eff_term_graph k t -> _ with
+  | TEffLast p b t' => fun G => match match_eff p b eff v with
+                                | Some f => Some (f (interpret_term_dep self (GTEffLast_inv G)))
+                                | None => None
+                                end
+  | TEffCons p b t1 t2 => fun G => match match_eff p b eff v with
+                                   | Some f => Some (f (interpret_term_dep self (GTEffCons_inv1 G)))
+                                   | None => interpret_eff_term_dep self (GTEffCons_inv2 G) eff v
+                                   end
   end G
-with interpret_ctx_clo_dep (self : interpreter) (k : kont) (c : ctx_clo) (G : ctx_clo_graph k c) (v : val) {struct G} : imonad iresult :=
-  match c return ctx_clo_graph k c -> imonad iresult with
-  | CCtx0 env t => fun G => imonad_use_env env (interpret_term_dep self (GCCtx0_inv G))
-  | CCtx1 env t => fun G => imonad_use_env env (interpret_term1_dep self (GCCtx1_inv G) v)
+with interpret_kont_clo_dep (self : interpreter) (k : kont) (c : kont_clo) (G : kont_clo_graph k c) (v : val) {struct G} : imonad iresult :=
+  match c return kont_clo_graph k c -> _ with
+  | CKSeq env t => fun G => imonad_use_env env (interpret_term_dep self (GCKSeq_inv G))
+  | CKLet env t => fun G => imonad_use_env env (interpret_term1_dep self (GCKLet_inv G) v)
   end G
 with interpret_kont_dep (self : interpreter) (k : kont) (G : kont_graph k) (v : val) {struct G} : imonad iresult :=
-  match k return kont_graph k -> imonad iresult with
-  | KNil => fun G => imonad_pure (RReturn v)
-  | KCons c k' => fun G => interpret_ctx_clo_dep self (GKCons_inv G) v
+  match k return kont_graph k -> _ with
+  | KNil => fun G => imonad_pure (RVal v)
+  | KCons c k' => fun G => interpret_kont_clo_dep self (GKCons_inv G) v
   end G.
 
 Unset Implicit Arguments.
@@ -778,7 +630,7 @@ Unset Implicit Arguments.
 Fixpoint build_kont_graph (k : kont) : kont_graph k :=
   match k with
   | KNil => GKNil
-  | KCons c k' => GKCons (build_ctx_clo_graph_dep (build_kont_graph k') c)
+  | KCons c k' => GKCons (build_kont_clo_graph_dep (build_kont_graph k') c)
   end.
 
 Definition build_term_graph (k : kont) (t : term) : term_graph k t :=
@@ -793,8 +645,17 @@ Fixpoint interpret_term (fuel : nat) (k : kont) (t : term) : imonad iresult :=
   | S fuel' => interpret_term_aux (interpret_term fuel') k t
   end.
 
+Definition unwrap_rval (r : iresult) : imonad val :=
+  match r with
+  | RVal v => imonad_pure v
+  | RShift _ _ tag => imonad_throw_error (Undelimited_shift tag)
+  | RControl _ _ tag => imonad_throw_error (Undelimited_control tag)
+  | RRaise exn => imonad_throw_error (Unhandled_exception exn)
+  | RPerform _ eff => imonad_throw_error (Unhandled_effect eff)
+  end.
+
 Definition run_term (fuel : nat) (t : term) : (ierror + val) * iheap :=
-  imonad_run (interpret_term fuel KNil t >>= unwrap_RReturn) EnvNil iheap_empty.
+  imonad_run (interpret_term fuel KNil t >>= unwrap_rval) EnvNil iheap_empty.
 
 Definition eval_term (fuel : nat) (t : term) : ierror + val :=
   fst (run_term fuel t).
