shift-reset/core/coerce.v
@@ -8,5 +8,4 @@ Coercion PVar : var >-> pattern.
 Coercion TVVar : var >-> val_term.
 Coercion TVInt : Z >-> val_term.
 Coercion TVFloat : Qc >-> val_term.
-Coercion TVBool : bool >-> val_term.
 Coercion TVal : val_term >-> term.
