shift-reset/core/val.v
@@ -1,6 +1,44 @@
+From Stdlib Require Import Qcanon ZArith.
 From shift_reset.core Require Import syntax tag.
 
-Definition VFun' (t : term1) (env : env) : val := VFun (CFun env t).
-Definition VFix' (t : term2) (env : env) : val := VFix (CFix env t).
-Definition VExn' (tag : tag) (v : val) : val := VExn (Exn tag v).
-Definition VEff' (tag : tag) (v : val) : val := VEff (Eff tag v).
+Definition VFun' (t : term1) (env : env) : val :=
+  VFun (CFun env t).
+
+Definition VFix' (t : term2) (env : env) : val :=
+  VFix (CFix env t).
+
+Definition VExn' (tag : tag) (v : val) : val :=
+  VExn (Exn tag v).
+
+Definition VEff' (tag : tag) (v : val) : val :=
+  VEff (Eff tag v).
+
+Definition VBool (b : bool) : val :=
+  if b then VTrue else VFalse.
+
+Definition VProd (p : val * val) : val :=
+  let (v1, v2) := p in VPair v1 v2.
+
+Definition VSum (s : val + val) : val :=
+  match s with
+  | inl v => VInl v
+  | inr v => VInr v
+  end.
+
+Definition VInt_by {A} (f : A -> Z) (x : A) : val :=
+  VInt (f x).
+
+Definition VFloat_by {A} (f : A -> Qc) (x : A) : val :=
+  VFloat (f x).
+
+Definition VBool_by {A} (f : A -> bool) (x : A) : val :=
+  VBool (f x).
+
+Definition VInt_by2 {A B} (f : A -> B -> Z) (x : A) (y : B) : val :=
+  VInt (f x y).
+
+Definition VFloat_by2 {A B} (f : A -> B -> Qc) (x : A) (y : B) : val :=
+  VFloat (f x y).
+
+Definition VBool_by2 {A B} (f : A -> B -> bool) (x : A) (y : B) : val :=
+  VBool (f x y).
