shift-reset/interpreter/iheap.v
@@ -1,23 +1,22 @@
-From Stdlib Require Import NArith.
 From shift_reset.lib Require option.
-From shift_reset.core Require Import heap syntax loc.
-
-Local Open Scope N_scope.
+From shift_reset.core Require Import syntax heap loc.
 
 Record iheap : Type := IHeap { iheap_car : heap; iheap_next_loc : loc }.
 
 Definition iheap_empty : iheap :=
-  IHeap heap_empty (Loc 0).
+  IHeap heap_empty loc_init.
 
 Definition iheap_ref (v : val) (h : iheap) : option (loc * iheap) :=
-  let l := iheap_next_loc h in
-  option.map (fun h' => (l, IHeap h' (loc_succ l))) (heap_ref l v (iheap_car h)).
+  let (h, l) := h in
+  option.map (fun h' => (l, IHeap h' (loc_succ l))) (heap_ref l v h).
 
 Definition iheap_get (l : loc) (h : iheap) : option val :=
   heap_get l (iheap_car h).
 
 Definition iheap_set (l : loc) (v : val) (h : iheap) : option iheap :=
-  option.map (fun h' => IHeap h' (iheap_next_loc h)) (heap_set l v (iheap_car h)).
+  let (h, l) := h in
+  option.map (fun h' => IHeap h' l) (heap_set l v h).
 
 Definition iheap_free (l : loc) (h : iheap) : option iheap :=
-  option.map (fun h' => IHeap h' (iheap_next_loc h)) (heap_free l (iheap_car h)).
+  let (h, l) := h in
+  option.map (fun h' => IHeap h' l) (heap_free l h).
