shift-reset/interpreter/unwrap.v
@@ -1,0 +1,79 @@
+From Stdlib Require Import String Qcanon ZArith.
+From shift_reset.core Require Import syntax loc tag.
+From shift_reset.interpreter Require Import ierror imonad.
+
+Local Open Scope string_scope.
+Local Unset Elimination Schemes.
+
+Inductive lambda : Type :=
+| LFun : fun_clo -> lambda
+| LFix : fix_clo -> lambda
+| LMKPure : metakont -> lambda
+| LMKReset : metakont -> tag -> lambda
+| LMKHandle : metakont -> handle_clo -> lambda.
+
+Definition unwrap_vunit (v : val) : imonad unit :=
+  match v with
+  | VUnit => imonad_pure tt
+  | _ => imonad_throw_error (Type_error "")
+  end.
+
+Definition unwrap_vint (v : val) : imonad Z :=
+  match v with
+  | VInt z => imonad_pure z
+  | _ => imonad_throw_error (Type_error "")
+  end.
+
+Definition unwrap_vfloat (v : val) : imonad Qc :=
+  match v with
+  | VFloat q => imonad_pure q
+  | _ => imonad_throw_error (Type_error "")
+  end.
+
+Definition unwrap_vbool (v : val) : imonad bool :=
+  match v with
+  | VTrue => imonad_pure true
+  | VFalse => imonad_pure false
+  | _ => imonad_throw_error (Type_error "")
+  end.
+
+Definition unwrap_vref (v : val) : imonad loc :=
+  match v with
+  | VRef l => imonad_pure l
+  | _ => imonad_throw_error (Type_error "")
+  end.
+
+Definition unwrap_vprod (v : val) : imonad (val * val) :=
+  match v with
+  | VPair v1 v2 => imonad_pure (v1, v2)
+  | _ => imonad_throw_error (Type_error "")
+  end.
+
+Definition unwrap_vsum (v : val) : imonad (val + val) :=
+  match v with
+  | VInl v' => imonad_pure (inl v')
+  | VInr v' => imonad_pure (inr v')
+  | _ => imonad_throw_error (Type_error "")
+  end.
+
+Definition unwrap_vexn (v : val) : imonad exn :=
+  match v with
+  | VExn exn => imonad_pure exn
+  | _ => imonad_throw_error (Type_error "")
+  end.
+
+Definition unwrap_veff (v : val) : imonad eff :=
+  match v with
+  | VEff eff => imonad_pure eff
+  | _ => imonad_throw_error (Type_error "")
+  end.
+
+Definition unwrap_vlambda (v : val) : imonad lambda :=
+  match v with
+  | VFun c => imonad_pure (LFun c)
+  | VFix c => imonad_pure (LFix c)
+  | VMKPure mk => imonad_pure (LMKPure mk)
+  | VMKReset mk tag => imonad_pure (LMKReset mk tag)
+  | VMKHandle mk c => imonad_pure (LMKHandle mk c)
+  | _ => imonad_throw_error (Type_error "")
+  end.
