shift-reset/lib/bool.v
@@ -1,0 +1,4 @@
+Definition bool_ltb (b1 b2 : bool) : bool := negb b1 && b2.
+Definition bool_leb (b1 b2 : bool) : bool := negb b1 || b2.
+Definition bool_gtb (b1 b2 : bool) : bool := b1 && negb b2.
+Definition bool_geb (b1 b2 : bool) : bool := b1 || negb b2.
