shift-reset/lib/comparison.v
@@ -1,0 +1,23 @@
+Definition compare_ltb (c : comparison) : bool :=
+  match c with
+  | Lt => true
+  | _ => false
+  end.
+
+Definition compare_leb (c : comparison) : bool :=
+  match c with
+  | Gt => false
+  | _ => true
+  end.
+
+Definition compare_gtb (c : comparison) : bool :=
+  match c with
+  | Gt => true
+  | _ => false
+  end.
+
+Definition compare_geb (c : comparison) : bool :=
+  match c with
+  | Lt => false
+  | _ => true
+  end.
