shift-reset/lib/int.v
@@ -1,0 +1,3 @@
+From Stdlib Require Import ZArith.
+
+Definition Z_neqb (z1 z2 : Z) : bool := negb (Z.eqb z1 z2).
